src/DICE.Core.fst
@@ -1,7 +1,6 @@
 /// Reference: https://github.com/microsoft/RIoT/blob/master/Reference/DICE/DiceCore.cpp
 module DICE.Core
 
-
 open LowStar.BufferOps
 open Lib.IntTypes
 open FStar.Integers
@@ -13,29 +12,14 @@ module I  = FStar.Integers
 module HI  = Lib.IntTypes
 
 module SHA2= Hacl.Hash.SHA2
-// module HMAC= Hacl.HMAC
-// module Ed25519 = Hacl.Ed25519
 
-// module CL  = C.Loops
-// module CE  = C.Endianness
-// module CF  = C.Failure
-// module C   = C
-// module CS  = C.String
-// module S   = FStar.Seq
-// module IB  = LowStar.ImmutableBuffer
 module B   = LowStar.Buffer
 module M   = LowStar.Modifies
 module HS  = FStar.HyperStack
 module HST = FStar.HyperStack.ST
 
-
-
-/// UDS type
-type uds_t (size: nat) = B.lbuffer HI.uint8 size
-
-/// CDI type, an alias of the hash digest type in Hacl*.
-type cdi_t (alg: hash_alg) = hash_t alg
-
+/// dice hash algorithm
+let _DICE_ALG = SHA2_256
 
 /// <><><><><><><><><><><><><><><><><><><><><><><><><><><><><><><><><><><>
 
@@ -45,39 +29,15 @@ assume val get_UDS
   (size: nat)
 : HST.Stack (b:B.buffer HI.uint8 {B.length b = size})
   (requires fun _ -> True)
-  (ensures  fun h0 uds h1 ->
-      B.live h1 uds)
+  (ensures  fun h0 result h1 ->
+      B.live h1 result)
 
-assume val get_Measurement
+assume val get_measurement
   (alg: hash_alg)
 : HST.Stack (hash_t alg)
   (requires fun _ -> True)
   (ensures  fun h0 r h1 ->
       B.live h1 r)
-
-/// REF: void DiceSHA256 (
-///        const uint8_t *buf,
-///        size_t bufSize,
-///        uint8_t *digest
-///      )
-assume val diceSHA256
-  (size : nat)
-  (data: B.lbuffer HI.uint8 size)
-  (digest: hash_t SHA2_256)
-: HST.Stack unit
-  (requires fun h ->
-      B.live h data
-    /\ B.live h digest
-    /\ B.disjoint data digest)
-  (ensures  fun h0 _ h1 ->
-      B.modifies (B.loc_buffer digest) h0 h1)
-///      {
-///          DICE_SHA256_CONTEXT context;
-///          DICE_SHA256_Init(&context);
-///          DICE_SHA256_Update(&context, buf, bufSize);
-///          DICE_SHA256_Final(&context, digest);
-///      }
-
 
 /// REF: void DiceSHA256_2 (
 ///        const uint8_t *buf1,
@@ -91,7 +51,7 @@ assume val diceSHA256_2
   (data1: B.lbuffer HI.uint8 size1)
   (size2 : nat)
   (data2 : B.lbuffer HI.uint8 size2)
-  (digest: hash_t SHA2_256)
+  (digest: hash_t _DICE_ALG)
 : HST.Stack unit
   (requires fun h ->
       B.live h data1
@@ -102,14 +62,6 @@ assume val diceSHA256_2
     /\ B.disjoint data2 digest)
   (ensures  fun h0 _ h1 ->
       B.modifies (B.loc_buffer digest) h0 h1)
-///      {
-///          DICE_SHA256_CONTEXT context;
-///          DICE_SHA256_Init(&context);
-///          DICE_SHA256_Update(&context, buf1, bufSize1);
-///          DICE_SHA256_Update(&context, buf2, bufSize2);
-///          DICE_SHA256_Final(&context, digest);
-///      }
-
 
 /// <><><><><><><><><><><><><><><><><><><><><><><><><><><><><><><><><><><>
 
@@ -118,46 +70,46 @@ assume val diceSHA256_2
 /// REF: #define DICE_UDS_LENGTH         0x20
 ///      #define DICE_DIGEST_LENGTH      0x20
 let _DICE_UDS_LENGTH    = 0x20
-let _DICE_DIGEST_LENGTH: uint_32 = hash_len SHA2_256
+let _DICE_DIGEST_LENGTH: uint_32 = hash_len _DICE_ALG
 
 
-/// <><><><><><><><><><><><><><><><><> DICE Core main funtion <><><><><><><><><><><><><><><><><><><
 
+/// <><><><><><><><><><><><> DICE Core main funtion <><><><><><><><><><><>
 
-#reset-options "--z3rlimit 50"
+#reset-options "--z3rlimit 10"
 let main ()
 : HST.Stack C.exit_code
-  (requires fun h -> True)
+  (requires fun _ -> True)
   (ensures  fun _ _ _ -> True)
 =
   HST.push_frame();
 
 /// NOTE: compute digest `uDigest` of `uds`
-  let uds : uds_t _DICE_UDS_LENGTH = get_UDS _DICE_UDS_LENGTH in
-  let uDigest :hash_t SHA2_256 = B.alloca (HI.u8 0x00) (hash_len SHA2_256) in
+  let uds : B.lbuffer uint8 _DICE_UDS_LENGTH = get_UDS _DICE_UDS_LENGTH in
+  let uDigest :hash_t _DICE_ALG = B.alloca (HI.u8 0x00) _DICE_DIGEST_LENGTH in
     SHA2.hash_256
       uds
       (u _DICE_UDS_LENGTH)
       uDigest;
 
 /// NOTE: compute digest `rDigest` of `measurement`
-  let measurement: hash_t SHA2_256 = get_Measurement SHA2_256 in
-  let rDigest :hash_t SHA2_256 = B.alloca (HI.u8 0x00) (hash_len SHA2_256) in
+  let measurement: hash_t _DICE_ALG = get_measurement _DICE_ALG in
+  let rDigest :hash_t _DICE_ALG = B.alloca (HI.u8 0x00) _DICE_DIGEST_LENGTH in
     SHA2.hash_256
       measurement
-      (hash_len SHA2_256)
+      _DICE_DIGEST_LENGTH
       rDigest;
 
-    let cdi: cdi_t SHA2_256
-      = B.alloca (HI.u8 0x00) (hash_len SHA2_256) in
+    let cdi: hash_t _DICE_ALG
+      = B.alloca (HI.u8 0x00) _DICE_DIGEST_LENGTH in
 
     diceSHA256_2
-     (v (hash_len SHA2_256)) uDigest
-     (v (hash_len SHA2_256)) rDigest
+     (v _DICE_DIGEST_LENGTH) uDigest
+     (v _DICE_DIGEST_LENGTH) rDigest
      cdi;
 
-    B.fill uDigest (HI.u8 0x00) (hash_len SHA2_256);
-    B.fill rDigest (HI.u8 0x00) (hash_len SHA2_256);
+    B.fill uDigest (HI.u8 0x00) _DICE_DIGEST_LENGTH;
+    B.fill rDigest (HI.u8 0x00) _DICE_DIGEST_LENGTH;
 
   HST.pop_frame();
   C.EXIT_SUCCESS
